more equations

src/lowparse/LowParse.Spec.VCList.fst
@@ -17,6 +17,42 @@ let parse_nlist
 : Tot (y: parser (parse_nlist_kind n k) (nlist n t) { y == parse_nlist' n p } )
 = parse_nlist' n p
 
+#push-options "--z3rlimit 32"
+#restart-solver
+
+let rec parse_nlist_sum
+  (#k: parser_kind)
+  (#t: Type)
+  (p: parser k t)
+  (n1 n2: nat)
+  (b: bytes)
+: Lemma
+  (ensures (parse (parse_nlist (n1 + n2) p) b ==
+    begin match parse (parse_nlist n1 p) b with
+    | None -> None
+    | Some (l1, consumed1) ->
+      let b2 = Seq.slice b consumed1 (Seq.length b) in
+      match parse (parse_nlist n2 p) b2 with
+      | None -> None
+      | Some (l2, consumed2) ->
+        List.Tot.append_length l1 l2;
+        Some (l1 `List.Tot.append` l2, consumed1 + consumed2)
+    end
+  ))
+  (decreases n1)
+= parse_nlist_eq n1 p b;
+  parse_nlist_eq (n1 + n2) p b;
+  if n1 = 0
+  then ()
+  else
+    match parse p b with
+    | None -> ()
+    | Some (x, consumed) ->
+      let b' = Seq.slice b consumed (Seq.length b) in
+      parse_nlist_sum p (n1 - 1) n2 b'
+
+#pop-options
+
 let serialize_nlist
   (n: nat)
   (#k: parser_kind)
